WP rules - load and store

theories/rules/rules_Load.v
@@ -14,60 +14,61 @@ Section cap_lang_rules.
   Implicit Types r : RegName.
   Implicit Types v : cap_lang.val. 
   Implicit Types w : Word.
-  Implicit Types reg : gmap RegName Word.
+  Implicit Types reg : gmap (CoreN * RegName) Word.
   Implicit Types ms : gmap Addr Word.
 
-  Definition reg_allows_load (regs : Reg) (r : RegName) p b e a  :=
-    regs !! r = Some (WCap p b e a) ∧
+  Definition reg_allows_load (regs : Reg) (i : CoreN) (r : RegName) p b e a  :=
+    regs !! (i, r) = Some (WCap p b e a) ∧
     readAllowed p = true ∧ withinBounds b e a = true.
 
-  Inductive Load_failure (regs: Reg) (r1 r2: RegName) (mem : gmap Addr Word) :=
+  Inductive Load_failure (i : CoreN) (regs: Reg) (r1 r2: RegName) (mem : gmap Addr Word) :=
   | Load_fail_const z:
-      regs !! r2 = Some (WInt z) ->
-      Load_failure regs r1 r2 mem
+      regs !! (i, r2) = Some (WInt z) ->
+      Load_failure i regs r1 r2 mem
   | Load_fail_bounds p b e a:
-      regs !! r2 = Some (WCap p b e a) ->
+      regs !! (i, r2) = Some (WCap p b e a) ->
       (readAllowed p = false ∨ withinBounds b e a = false) →
-      Load_failure regs r1 r2 mem
+      Load_failure i regs r1 r2 mem
   (* Notice how the None below also includes all cases where we read an inl value into the PC, because then incrementing it will fail *)
   | Load_fail_invalid_PC p b e a loadv:
-      regs !! r2 = Some (WCap p b e a) ->
+      regs !! (i, r2) = Some (WCap p b e a) ->
       mem !! a = Some loadv →
-      incrementPC (<[ r1 := loadv ]> regs) = None ->
-      Load_failure regs r1 r2 mem
+      incrementPC (<[ (i, r1) := loadv ]> regs) i = None ->
+      Load_failure i regs r1 r2 mem
   .
 
   Inductive Load_spec
+    (i : CoreN)
     (regs: Reg) (r1 r2: RegName)
     (regs': Reg) (mem : gmap Addr Word) : cap_lang.val → Prop
   :=
   | Load_spec_success p b e a loadv :
-    reg_allows_load regs r2 p b e a →
+    reg_allows_load regs i r2 p b e a →
     mem !! a = Some loadv →
     incrementPC
-      (<[ r1 := loadv ]> regs) = Some regs' ->
-    Load_spec regs r1 r2 regs' mem NextIV
+      (<[ (i, r1) := loadv ]> regs) i = Some regs' ->
+    Load_spec i regs r1 r2 regs' mem (i, NextIV)
 
   | Load_spec_failure :
-    Load_failure regs r1 r2 mem ->
-    Load_spec regs r1 r2 regs' mem FailedV.
+    Load_failure i regs r1 r2 mem ->
+    Load_spec i regs r1 r2 regs' mem (i, FailedV).
 
-  Definition allow_load_map_or_true r (regs : Reg) (mem : gmap Addr Word):=
-    ∃ p b e a, read_reg_inr regs r p b e a ∧
-      if decide (reg_allows_load regs r p b e a) then
+  Definition allow_load_map_or_true (i : CoreN) r (regs : Reg) (mem : gmap Addr Word):=
+    ∃ p b e a, read_reg_inr regs i r p b e a ∧
+      if decide (reg_allows_load regs i r p b e a) then
         ∃ w, mem !! a = Some w 
       else True.
 
   Lemma allow_load_implies_loadv:
-    ∀ (r2 : RegName) (mem0 : gmap Addr Word) (r : Reg) (p : Perm) (b e a : Addr),
-      allow_load_map_or_true r2 r mem0
-      → r !! r2 = Some (WCap p b e a)
+    ∀ (i : CoreN) (r2 : RegName) (mem0 : gmap Addr Word) (r : Reg) (p : Perm) (b e a : Addr),
+      allow_load_map_or_true i r2 r mem0
+      → r !! (i, r2) = Some (WCap p b e a)
       → readAllowed p = true
       → withinBounds b e a = true
       → ∃ (loadv : Word),
           mem0 !! a = Some loadv.
   Proof.
-    intros r2 mem0 r p b e a HaLoad Hr2v Hra Hwb.
+    intros i r2 mem0 r p b e a HaLoad Hr2v Hra Hwb.
     unfold allow_load_map_or_true in HaLoad.
     destruct HaLoad as (?&?&?&?&[Hrr | Hrl]&Hmem).
     - assert (Hrr' := Hrr). rewrite Hrr in Hr2v; inversion Hr2v; subst.
@@ -79,43 +80,43 @@ Section cap_lang_rules.
   Qed.
 
   Lemma mem_eq_implies_allow_load_map:
-    ∀ (regs : Reg)(mem : gmap Addr Word)(r2 : RegName) (w : Word) p b e a,
+    ∀ (i : CoreN) (regs : Reg)(mem : gmap Addr Word)(r2 : RegName) (w : Word) p b e a,
       mem = <[a:=w]> ∅
-      → regs !! r2 = Some (WCap p b e a)
-      → allow_load_map_or_true r2 regs mem.
+      → regs !! (i, r2) = Some (WCap p b e a)
+      → allow_load_map_or_true i r2 regs mem.
   Proof.
-    intros regs mem r2 w p b e a Hmem Hrr2.
+    intros i regs mem r2 w p b e a Hmem Hrr2.
     exists p,b,e,a; split.
-    - left. by simplify_map_eq.
+    - left. by simplify_map_eq by simplify_pair_eq.
     - case_decide; last done.
-      exists w. simplify_map_eq. auto.
+      exists w. simplify_map_eq by simplify_pair_eq. auto.
   Qed.
 
   Lemma mem_neq_implies_allow_load_map:
-    ∀ (regs : Reg)(mem : gmap Addr Word)(r2 : RegName) (pc_a : Addr)
+    ∀ (i : CoreN) (regs : Reg)(mem : gmap Addr Word)(r2 : RegName) (pc_a : Addr)
       (w w' : Word) p b e a,
       a ≠ pc_a
       → mem = <[pc_a:=w]> (<[a:=w']> ∅)
-      → regs !! r2 = Some (WCap p b e a)
-      → allow_load_map_or_true r2 regs mem.
+      → regs !! (i, r2) = Some (WCap p b e a)
+      → allow_load_map_or_true i r2 regs mem.
   Proof.
-    intros regs mem r2 pc_a w w' p b e a H4 Hrr2.
+    intros i regs mem r2 pc_a w w' p b e a H4 Hrr2.
     exists p,b,e,a; split.
-    - left. by simplify_map_eq.
+    - left. by simplify_map_eq by simplify_pair_eq.
     - case_decide; last done.
-      exists w'. simplify_map_eq. split; auto.
+      exists w'. simplify_map_eq by simplify_pair_eq. split; auto.
   Qed.
 
   Lemma mem_implies_allow_load_map:
-    ∀ (regs : Reg)(mem : gmap Addr Word)(r2 : RegName) (pc_a : Addr)
+    ∀ (i : CoreN) (regs : Reg)(mem : gmap Addr Word)(r2 : RegName) (pc_a : Addr)
       (w w' : Word) p b e a,
       (if (a =? pc_a)%a
        then mem = <[pc_a:=w]> ∅
        else mem = <[pc_a:=w]> (<[a:=w']> ∅))
-      → regs !! r2 = Some (WCap p b e a)
-      → allow_load_map_or_true r2 regs mem.
+      → regs !! (i, r2) = Some (WCap p b e a)
+      → allow_load_map_or_true i r2 regs mem.
   Proof.
-    intros regs mem r2 pc_a w w' p b e a H4 Hrr2.
+    intros i regs mem r2 pc_a w w' p b e a H4 Hrr2.
     destruct (a =? pc_a)%a eqn:Heq.
       + apply Z.eqb_eq, finz_to_z_eq in Heq. subst a. eapply mem_eq_implies_allow_load_map; eauto.
       + apply Z.eqb_neq in Heq. eapply mem_neq_implies_allow_load_map; eauto. congruence.
@@ -132,8 +133,8 @@ Section cap_lang_rules.
   Proof.
     intros pc_a w w' a0 mem0 loadv H4 H6.
     destruct (a0 =? pc_a)%a eqn:Heq; rewrite H4 in H6.
-    + apply Z.eqb_eq, finz_to_z_eq in Heq; subst a0. by simplify_map_eq.
-    + apply Z.eqb_neq in Heq. rewrite lookup_insert_ne in H6; last congruence. by simplify_map_eq.
+    + apply Z.eqb_eq, finz_to_z_eq in Heq; subst a0. by simplify_map_eq by simplify_pair_eq.
+    + apply Z.eqb_neq in Heq. rewrite lookup_insert_ne in H6; last congruence. by simplify_map_eq by simplify_pair_eq.
   Qed.
 
   (* a more general version of load to work also with any fraction and persistent points tos *)
@@ -164,22 +165,22 @@ Section cap_lang_rules.
   Instance prod_op_DiagNone {A B : Type} : (DiagNone (@prod_op A B)).
   Proof. cbv. auto. Qed.
 
-  Lemma wp_load_general Ep
+  Lemma wp_load_general Ep i
      pc_p pc_b pc_e pc_a
      r1 r2 w mem (dfracs : gmap Addr dfrac) regs :
    decodeInstrW w = Load r1 r2 →
    isCorrectPC (WCap pc_p pc_b pc_e pc_a) →
-   regs !! PC = Some (WCap pc_p pc_b pc_e pc_a) →
-   regs_of (Load r1 r2) ⊆ dom _ regs →
+   regs !! (i, PC) = Some (WCap pc_p pc_b pc_e pc_a) →
+   regs_of_core (Load r1 r2) i ⊆ dom _ regs →
    mem !! pc_a = Some w →
-   allow_load_map_or_true r2 regs mem →
+   allow_load_map_or_true i r2 regs mem →
    dom (gset Addr) mem = dom (gset Addr) dfracs →
 
    {{{ (▷ [∗ map] a↦dw ∈ prod_merge dfracs mem, a ↦ₐ{dw.1} dw.2) ∗
        ▷ [∗ map] k↦y ∈ regs, k ↦ᵣ y }}}
-     Instr Executable @ Ep
+     (i, Instr Executable) @ Ep
    {{{ regs' retv, RET retv;
-       ⌜ Load_spec regs r1 r2 regs' mem retv⌝ ∗
+       ⌜ Load_spec i regs r1 r2 regs' mem retv⌝ ∗
          ([∗ map] a↦dw ∈ prod_merge dfracs mem, a ↦ₐ{dw.1} dw.2) ∗
          [∗ map] k↦y ∈ regs', k ↦ᵣ y }}}.
   Proof.
@@ -190,9 +191,9 @@ Section cap_lang_rules.
 
     (* Derive necessary register values in r *)
     pose proof (lookup_weaken _ _ _ _ HPC Hregs).
-    specialize (indom_regs_incl _ _ _ Dregs Hregs) as Hri. unfold regs_of in Hri.
-    feed destruct (Hri r2) as [r2v [Hr'2 Hr2]]. by set_solver+.
-    feed destruct (Hri r1) as [r1v [Hr'1 _]]. by set_solver+. clear Hri.
+    specialize (indom_regs_incl _ _ _ Dregs Hregs) as Hri. unfold regs_of_core in Hri.
+    feed destruct (Hri i r2) as [r2v [Hr'2 Hr2]]. by set_solver+.
+    feed destruct (Hri i r1) as [r1v [Hr'1 _]]. by set_solver+. clear Hri.
     (* Derive the PC in memory *)
     assert (is_Some (dfracs !! pc_a)) as [dq Hdq].
     { apply elem_of_gmap_dom. rewrite -Hdomeq. apply elem_of_gmap_dom;eauto. }
@@ -204,7 +205,7 @@ Section cap_lang_rules.
     iSplitR. by iPureIntro; apply normal_always_head_reducible.
     iNext. iIntros (e2 σ2 efs Hpstep).
     apply prim_step_exec_inv in Hpstep as (-> & -> & (c & -> & Hstep)).
-    iSplitR; auto. eapply step_exec_inv in Hstep; eauto.
+    iSplitR; auto. eapply core_step_exec_inv in Hstep; eauto.
 
     unfold exec in Hstep; simpl in Hstep. rewrite Hr2 in Hstep.
 
@@ -225,7 +226,7 @@ Section cap_lang_rules.
     apply andb_true_iff in HRA; destruct HRA as (Hra & Hwb).
 
     (* Prove that a is in the memory map now, otherwise we cannot continue *)
-    pose proof (allow_load_implies_loadv r2 mem regs p b e a) as (loadv & Hmema); auto.
+    pose proof (allow_load_implies_loadv i r2 mem regs p b e a) as (loadv & Hmema); auto.
 
     assert (is_Some (dfracs !! a)) as [dq' Hdq'].
     { apply elem_of_gmap_dom. rewrite -Hdomeq. apply elem_of_gmap_dom;eauto. }
@@ -234,9 +235,9 @@ Section cap_lang_rules.
     iDestruct (gen_mem_valid_inSepM_general (prod_merge dfracs mem) m a loadv with "Hm Hmem" ) as %Hma' ; eauto.
 
     rewrite Hma' /= in Hstep.
-    destruct (incrementPC (<[ r1 := loadv ]> regs)) as  [ regs' |] eqn:Hregs'.
+    destruct (incrementPC (<[ (i, r1) := loadv ]> regs) i) as  [ regs' |] eqn:Hregs'.
     2: { (* Failure: the PC could not be incremented correctly *)
-      assert (incrementPC (<[ r1 := loadv]> r) = None).
+      assert (incrementPC (<[ (i, r1) := loadv]> r) i = None).
       { eapply incrementPC_overflow_mono; first eapply Hregs'.
           by rewrite lookup_insert_is_Some'; eauto.
             by apply insert_mono; eauto. }
@@ -249,13 +250,13 @@ Section cap_lang_rules.
 
     (* Success *)
     rewrite /update_reg /= in Hstep.
-    eapply (incrementPC_success_updatePC _ m) in Hregs'
+    eapply (incrementPC_success_updatePC _ i m) in Hregs'
       as (p1 & b1 & e1 & a1 & a_pc1 & HPC'' & Ha_pc' & HuPC & ->).
     eapply updatePC_success_incl in HuPC. 2: by eapply insert_mono.
     rewrite HuPC in Hstep; clear HuPC; inversion Hstep; clear Hstep; subst c σ2. cbn.
     iFrame.
-    iMod ((gen_heap_update_inSepM _ _ r1) with "Hr Hmap") as "[Hr Hmap]"; eauto.
-    iMod ((gen_heap_update_inSepM _ _ PC) with "Hr Hmap") as "[Hr Hmap]"; eauto.
+    iMod ((gen_heap_update_inSepM _ _ (i, r1)) with "Hr Hmap") as "[Hr Hmap]"; eauto.
+    iMod ((gen_heap_update_inSepM _ _ (i, PC)) with "Hr Hmap") as "[Hr Hmap]"; eauto.
     iFrame. iModIntro. iApply "Hφ". iFrame.
     iPureIntro. eapply Load_spec_success; auto.
     * split; eauto.
@@ -316,21 +317,21 @@ Section cap_lang_rules.
         iFrame. iApply "IH". iFrame.
   Qed.
 
-  Lemma wp_load Ep
+  Lemma wp_load Ep i
      pc_p pc_b pc_e pc_a
      r1 r2 w mem regs dq :
    decodeInstrW w = Load r1 r2 →
    isCorrectPC (WCap pc_p pc_b pc_e pc_a) →
-   regs !! PC = Some (WCap pc_p pc_b pc_e pc_a) →
-   regs_of (Load r1 r2) ⊆ dom _ regs →
+   regs !! (i, PC) = Some (WCap pc_p pc_b pc_e pc_a) →
+   regs_of_core (Load r1 r2) i ⊆ dom _ regs →
    mem !! pc_a = Some w →
-   allow_load_map_or_true r2 regs mem →
+   allow_load_map_or_true i r2 regs mem →
 
    {{{ (▷ [∗ map] a↦w ∈ mem, a ↦ₐ{dq} w) ∗
        ▷ [∗ map] k↦y ∈ regs, k ↦ᵣ y }}}
-     Instr Executable @ Ep
+     (i, Instr Executable) @ Ep
    {{{ regs' retv, RET retv;
-       ⌜ Load_spec regs r1 r2 regs' mem retv⌝ ∗
+       ⌜ Load_spec i regs r1 r2 regs' mem retv⌝ ∗
          ([∗ map] a↦w ∈ mem, a ↦ₐ{dq} w) ∗
          [∗ map] k↦y ∈ regs', k ↦ᵣ y }}}.
   Proof.
@@ -394,23 +395,23 @@ Section cap_lang_rules.
       iDestruct (big_sepM_insert with "Hmem") as "[$ Hmem]". auto.
   Qed.
 
-  Lemma wp_load_success E r1 r2 pc_p pc_b pc_e pc_a w w' w'' p b e a pc_a' dq dq' :
+  Lemma wp_load_success E i r1 r2 pc_p pc_b pc_e pc_a w w' w'' p b e a pc_a' dq dq' :
     decodeInstrW w = Load r1 r2 →
     isCorrectPC (WCap pc_p pc_b pc_e pc_a) →
     readAllowed p = true ∧ withinBounds b e a = true →
     (pc_a + 1)%a = Some pc_a' →
 
-    {{{ ▷ PC ↦ᵣ WCap pc_p pc_b pc_e pc_a
+    {{{ ▷ (i, PC) ↦ᵣ WCap pc_p pc_b pc_e pc_a
           ∗ ▷ pc_a ↦ₐ{dq} w
-          ∗ ▷ r1 ↦ᵣ w''
-          ∗ ▷ r2 ↦ᵣ WCap p b e a
+          ∗ ▷ (i, r1) ↦ᵣ w''
+          ∗ ▷ (i, r2) ↦ᵣ WCap p b e a
           ∗ (if (eqb_addr a pc_a) then emp else ▷ a ↦ₐ{dq'} w') }}}
-      Instr Executable @ E
-      {{{ RET NextIV;
-          PC ↦ᵣ WCap pc_p pc_b pc_e pc_a'
-             ∗ r1 ↦ᵣ (if (eqb_addr a pc_a) then w else w')
+      (i, Instr Executable) @ E
+      {{{ RET (i, NextIV);
+          (i, PC) ↦ᵣ WCap pc_p pc_b pc_e pc_a'
+             ∗ (i, r1) ↦ᵣ (if (eqb_addr a pc_a) then w else w')
              ∗ pc_a ↦ₐ{dq} w
-             ∗ r2 ↦ᵣ WCap p b e a
+             ∗ (i, r2) ↦ᵣ WCap p b e a
              ∗ (if (eqb_addr a pc_a) then emp else a ↦ₐ{dq'} w') }}}.
   Proof.
     iIntros (Hinstr Hvpc [Hra Hwb] Hpca' φ)
@@ -419,10 +420,11 @@ Section cap_lang_rules.
     iDestruct (memMap_resource_2gen_clater_dq _ _ _ _ _ _ (λ a dq w, a ↦ₐ{dq} w)%I with "Hi Hr2a") as (mem dfracs) "[>Hmem Hmem']".
     iDestruct "Hmem'" as %[Hmem Hdfracs].
 
-    iApply (wp_load_general with "[$Hmap $Hmem]"); eauto; simplify_map_eq; eauto.
+    iApply (wp_load_general with "[$Hmap $Hmem]"); eauto; simplify_map_eq by simplify_pair_eq; eauto.
     { by rewrite !dom_insert; set_solver+. }
-    { destruct (a =? pc_a)%a; by simplify_map_eq. }
-    { eapply mem_implies_allow_load_map; eauto. by simplify_map_eq. }
+    { destruct (a =? pc_a)%a; by simplify_map_eq by simplify_pair_eq. }
+    { eapply mem_implies_allow_load_map; eauto.
+      by simplify_map_eq by simplify_pair_eq. }
     { destruct (a =? pc_a)%a; simplify_eq. all: rewrite !dom_insert_L;set_solver+. }
     iNext. iIntros (regs' retv) "(#Hspec & Hmem & Hmap)".
     iDestruct "Hspec" as %Hspec.
@@ -430,37 +432,39 @@ Section cap_lang_rules.
     destruct Hspec as [ | * Hfail ].
      { (* Success *)
        (* FIXME: fragile *)
-       destruct H5 as [Hrr2 _]. simplify_map_eq.
+       destruct H5 as [Hrr2 _]. simplify_map_eq by simplify_pair_eq.
        iDestruct (memMap_resource_2gen_d_dq with "[Hmem]") as "[Hpc_a Ha]".
        { iExists mem,dfracs; iSplitL; auto. }
        incrementPC_inv.
        pose proof (mem_implies_loadv _ _ _ _ _ _ Hmem H6) as Hloadv; eauto.
-       simplify_map_eq.
-       rewrite (insert_commute _ PC r1) // insert_insert (insert_commute _ r1 PC) // insert_insert.
+       simplify_map_eq by simplify_pair_eq.
+       rewrite (insert_commute _ (i, PC) (i, r1)) ; simplify_pair_eq.
+       rewrite insert_insert (insert_commute _ (i, r1) (i, PC)) ; simplify_pair_eq.
+       rewrite insert_insert ; simplify_pair_eq.
        iDestruct (regs_of_map_3 with "[$Hmap]") as "[HPC [Hr1 Hr2] ]"; eauto.
        iApply "Hφ". iFrame. }
      { (* Failure (contradiction) *)
-       destruct Hfail; try incrementPC_inv; simplify_map_eq; eauto.
+       destruct Hfail; try incrementPC_inv; simplify_map_eq by simplify_pair_eq; eauto.
        destruct o. all: congruence. }
   Qed.
 
-  Lemma wp_load_success_notinstr E r1 r2 pc_p pc_b pc_e pc_a w w' w'' p b e a pc_a' dq dq' :
+  Lemma wp_load_success_notinstr E i r1 r2 pc_p pc_b pc_e pc_a w w' w'' p b e a pc_a' dq dq' :
     decodeInstrW w = Load r1 r2 →
     isCorrectPC (WCap pc_p pc_b pc_e pc_a) →
     readAllowed p = true ∧ withinBounds b e a = true →
     (pc_a + 1)%a = Some pc_a' →
 
-    {{{ ▷ PC ↦ᵣ WCap pc_p pc_b pc_e pc_a
+    {{{ ▷ (i, PC) ↦ᵣ WCap pc_p pc_b pc_e pc_a
           ∗ ▷ pc_a ↦ₐ{dq} w
-          ∗ ▷ r1 ↦ᵣ w''
-          ∗ ▷ r2 ↦ᵣ WCap p b e a
+          ∗ ▷ (i, r1) ↦ᵣ w''
+          ∗ ▷ (i, r2) ↦ᵣ WCap p b e a
           ∗ ▷ a ↦ₐ{dq'} w' }}}
-      Instr Executable @ E
-      {{{ RET NextIV;
-          PC ↦ᵣ WCap pc_p pc_b pc_e pc_a'
-             ∗ r1 ↦ᵣ w'
+      (i, Instr Executable) @ E
+      {{{ RET (i, NextIV);
+          (i, PC) ↦ᵣ WCap pc_p pc_b pc_e pc_a'
+             ∗ (i, r1) ↦ᵣ w'
              ∗ pc_a ↦ₐ{dq} w
-             ∗ r2 ↦ᵣ WCap p b e a
+             ∗ (i, r2) ↦ᵣ WCap p b e a
              ∗ a ↦ₐ{dq'} w' }}}.
   Proof.
     intros. iIntros "(>HPC & >Hpc_a & >Hr1 & >Hr2 & >Ha)".
@@ -478,22 +482,22 @@ Section cap_lang_rules.
     iApply "Hφ". iFrame. Unshelve. apply DfracDiscarded. apply (WInt 0).
   Qed.
 
-  Lemma wp_load_success_frominstr E r1 r2 pc_p pc_b pc_e pc_a w w'' p b e pc_a' dq :
+  Lemma wp_load_success_frominstr E i r1 r2 pc_p pc_b pc_e pc_a w w'' p b e pc_a' dq :
     decodeInstrW w = Load r1 r2 →
     isCorrectPC (WCap pc_p pc_b pc_e pc_a) →
     readAllowed p = true ∧ withinBounds b e pc_a = true →
     (pc_a + 1)%a = Some pc_a' →
 
-    {{{ ▷ PC ↦ᵣ WCap pc_p pc_b pc_e pc_a
+    {{{ ▷ (i, PC) ↦ᵣ WCap pc_p pc_b pc_e pc_a
           ∗ ▷ pc_a ↦ₐ{dq} w
-          ∗ ▷ r1 ↦ᵣ w''
-          ∗ ▷ r2 ↦ᵣ WCap p b e pc_a }}}
-      Instr Executable @ E
-      {{{ RET NextIV;
-          PC ↦ᵣ WCap pc_p pc_b pc_e pc_a'
-             ∗ r1 ↦ᵣ w
+          ∗ ▷ (i, r1) ↦ᵣ w''
+          ∗ ▷ (i, r2) ↦ᵣ WCap p b e pc_a }}}
+      (i, Instr Executable) @ E
+      {{{ RET (i, NextIV);
+          (i, PC) ↦ᵣ WCap pc_p pc_b pc_e pc_a'
+             ∗ (i, r1) ↦ᵣ w
              ∗ pc_a ↦ₐ{dq} w
-             ∗ r2 ↦ᵣ WCap p b e pc_a }}}.
+             ∗ (i, r2) ↦ᵣ WCap p b e pc_a }}}.
   Proof.
     intros. iIntros "(>HPC & >Hpc_a & >Hr1 & >Hr2)".
     iIntros "Hφ". iApply (wp_load_success with "[$HPC $Hpc_a $Hr1 $Hr2]"); eauto.
@@ -502,21 +506,21 @@ Section cap_lang_rules.
     iApply "Hφ". iFrame. Unshelve. all: eauto.
   Qed.
 
-  Lemma wp_load_success_same E r1 pc_p pc_b pc_e pc_a w w' w'' p b e a pc_a' dq dq' :
+  Lemma wp_load_success_same E i r1 pc_p pc_b pc_e pc_a w w' w'' p b e a pc_a' dq dq' :
     decodeInstrW w = Load r1 r1 →
     isCorrectPC (WCap pc_p pc_b pc_e pc_a) →
     readAllowed p = true →
     withinBounds b e a = true →
     (pc_a + 1)%a = Some pc_a' →
 
-    {{{ ▷ PC ↦ᵣ WCap pc_p pc_b pc_e pc_a
+    {{{ ▷ (i, PC) ↦ᵣ WCap pc_p pc_b pc_e pc_a
           ∗ ▷ pc_a ↦ₐ{dq} w
-          ∗ ▷ r1 ↦ᵣ WCap p b e a
+          ∗ ▷ (i, r1) ↦ᵣ WCap p b e a
           ∗ (if (a =? pc_a)%a then emp else ▷ a ↦ₐ{dq'} w') }}}
-      Instr Executable @ E
-      {{{ RET NextIV;
-          PC ↦ᵣ WCap pc_p pc_b pc_e pc_a'
-             ∗ r1 ↦ᵣ (if (a =? pc_a)%a then w else w')
+      (i, Instr Executable) @ E
+      {{{ RET (i, NextIV);
+          (i, PC) ↦ᵣ WCap pc_p pc_b pc_e pc_a'
+             ∗ (i, r1) ↦ᵣ (if (a =? pc_a)%a then w else w')
              ∗ pc_a ↦ₐ{dq} w
              ∗ (if (a =? pc_a)%a then emp else a ↦ₐ{dq'} w') }}}.
   Proof.
@@ -527,10 +531,10 @@ Section cap_lang_rules.
         (mem dfracs) "[>Hmem Hmem']".
     iDestruct "Hmem'" as %[Hmem Hfracs].
 
-    iApply (wp_load_general with "[$Hmap $Hmem]"); eauto; simplify_map_eq; eauto.
+    iApply (wp_load_general with "[$Hmap $Hmem]"); eauto; simplify_map_eq by simplify_pair_eq; eauto.
     { by rewrite !dom_insert; set_solver+. }
-    { destruct (a =? pc_a)%a; by simplify_map_eq. }
-    { eapply mem_implies_allow_load_map; eauto. by simplify_map_eq. }
+    { destruct (a =? pc_a)%a; by simplify_map_eq by simplify_pair_eq. }
+    { eapply mem_implies_allow_load_map; eauto. by simplify_map_eq by simplify_pair_eq. }
     { destruct (a =? pc_a)%a; by set_solver. }
     iNext. iIntros (regs' retv) "(#Hspec & Hmem & Hmap)".
     iDestruct "Hspec" as %Hspec.
@@ -538,34 +542,36 @@ Section cap_lang_rules.
     destruct Hspec as [ | * Hfail ].
      { (* Success *)
        iApply "Hφ".
-       destruct H3 as [Hrr2 _]. simplify_map_eq.
+       destruct H3 as [Hrr2 _]. simplify_map_eq by simplify_pair_eq.
        iDestruct (memMap_resource_2gen_d_dq with "[Hmem]") as "[Hpc_a Ha]".
        {iExists mem,dfracs; iSplitL; auto. }
        incrementPC_inv.
        pose proof (mem_implies_loadv _ _ _ _ _ _ Hmem H4) as Hloadv; eauto.
-       simplify_map_eq.
-       rewrite (insert_commute _ PC r1) // insert_insert (insert_commute _ r1 PC) // insert_insert.
+       simplify_map_eq by simplify_pair_eq.
+       rewrite (insert_commute _ (i, PC) (i, r1)) ; simplify_pair_eq.
+       rewrite insert_insert (insert_commute _ (i, r1) (i, PC)) ; simplify_pair_eq.
+       rewrite insert_insert ; simplify_pair_eq.
        iDestruct (regs_of_map_2 with "[$Hmap]") as "[HPC Hr1]"; eauto. iFrame. }
      { (* Failure (contradiction) *)
-       destruct Hfail; try incrementPC_inv; simplify_map_eq; eauto.
+       destruct Hfail; try incrementPC_inv; simplify_map_eq by simplify_pair_eq; eauto.
        destruct o. all: congruence. }
     Qed.
 
-  Lemma wp_load_success_same_notinstr E r1 pc_p pc_b pc_e pc_a w w' w'' p b e a pc_a' dq dq' :
+  Lemma wp_load_success_same_notinstr E i r1 pc_p pc_b pc_e pc_a w w' w'' p b e a pc_a' dq dq' :
     decodeInstrW w = Load r1 r1 →
     isCorrectPC (WCap pc_p pc_b pc_e pc_a) →
     readAllowed p = true →
     withinBounds b e a = true →
     (pc_a + 1)%a = Some pc_a' →
 
-    {{{ ▷ PC ↦ᵣ WCap pc_p pc_b pc_e pc_a
+    {{{ ▷ (i, PC) ↦ᵣ WCap pc_p pc_b pc_e pc_a
           ∗ ▷ pc_a ↦ₐ{dq} w
-          ∗ ▷ r1 ↦ᵣ WCap p b e a
+          ∗ ▷ (i, r1) ↦ᵣ WCap p b e a
           ∗ ▷ a ↦ₐ{dq'} w' }}}
-      Instr Executable @ E
-      {{{ RET NextIV;
-          PC ↦ᵣ WCap pc_p pc_b pc_e pc_a'
-             ∗ r1 ↦ᵣ w'
+      (i, Instr Executable) @ E
+      {{{ RET (i, NextIV);
+          (i, PC) ↦ᵣ WCap pc_p pc_b pc_e pc_a'
+             ∗ (i, r1) ↦ᵣ w'
              ∗ pc_a ↦ₐ{dq} w
              ∗ a ↦ₐ{dq'} w' }}}.
   Proof.
@@ -585,20 +591,20 @@ Section cap_lang_rules.
     iApply "Hφ". iFrame. Unshelve. apply (WInt 0). apply DfracDiscarded.
   Qed.
 
-  Lemma wp_load_success_same_frominstr E r1 pc_p pc_b pc_e pc_a w p b e pc_a' dq :
+  Lemma wp_load_success_same_frominstr E i r1 pc_p pc_b pc_e pc_a w p b e pc_a' dq :
     decodeInstrW w = Load r1 r1 →
     isCorrectPC (WCap pc_p pc_b pc_e pc_a) →
     readAllowed p = true →
     withinBounds b e pc_a = true →
     (pc_a + 1)%a = Some pc_a' →
 
-    {{{ ▷ PC ↦ᵣ WCap pc_p pc_b pc_e pc_a
+    {{{ ▷ (i, PC) ↦ᵣ WCap pc_p pc_b pc_e pc_a
           ∗ ▷ pc_a ↦ₐ{dq} w
-          ∗ ▷ r1 ↦ᵣ WCap p b e pc_a }}}
-      Instr Executable @ E
-      {{{ RET NextIV;
-          PC ↦ᵣ WCap pc_p pc_b pc_e pc_a'
-             ∗ r1 ↦ᵣ w
+          ∗ ▷ (i, r1) ↦ᵣ WCap p b e pc_a }}}
+      (i, Instr Executable) @ E
+      {{{ RET (i, NextIV);
+          (i, PC) ↦ᵣ WCap pc_p pc_b pc_e pc_a'
+             ∗ (i, r1) ↦ᵣ w
              ∗ pc_a ↦ₐ{dq} w }}}.
   Proof.
     intros. iIntros "(>HPC & >Hpc_a & >Hr1)".
@@ -609,46 +615,46 @@ Section cap_lang_rules.
   Qed.
 
   (* If a points to a capability, the load into PC success if its address can be incr *)
-  Lemma wp_load_success_PC E r2 pc_p pc_b pc_e pc_a w
+  Lemma wp_load_success_PC E i r2 pc_p pc_b pc_e pc_a w
         p b e a p' b' e' a' a'' :
     decodeInstrW w = Load PC r2 →
     isCorrectPC (WCap pc_p pc_b pc_e pc_a) →
     readAllowed p = true ∧ withinBounds b e a = true →
     (a' + 1)%a = Some a'' →
 
-    {{{ ▷ PC ↦ᵣ WCap pc_p pc_b pc_e pc_a
+    {{{ ▷ (i, PC) ↦ᵣ WCap pc_p pc_b pc_e pc_a
           ∗ ▷ pc_a ↦ₐ w
-          ∗ ▷ r2 ↦ᵣ WCap p b e a
+          ∗ ▷ (i, r2) ↦ᵣ WCap p b e a
           ∗ ▷ a ↦ₐ WCap p' b' e' a' }}}
-      Instr Executable @ E
-      {{{ RET NextIV;
-          PC ↦ᵣ WCap p' b' e' a''
+      (i, Instr Executable) @ E
+      {{{ RET (i, NextIV);
+          (i, PC) ↦ᵣ WCap p' b' e' a''
              ∗ pc_a ↦ₐ w
-             ∗ r2 ↦ᵣ WCap p b e a
+             ∗ (i, r2) ↦ᵣ WCap p b e a
              ∗ a ↦ₐ WCap p' b' e' a' }}}.
   Proof.
     iIntros (Hinstr Hvpc [Hra Hwb] Hpca' φ)
             "(>HPC & >Hi & >Hr2 & >Hr2a) Hφ".
     iDestruct (map_of_regs_2 with "HPC Hr2") as "[Hmap %]".
     iDestruct (memMap_resource_2ne_apply with "Hi Hr2a") as "[Hmem %]"; auto.
-    iApply (wp_load with "[$Hmap $Hmem]"); eauto; simplify_map_eq; eauto.
+    iApply (wp_load with "[$Hmap $Hmem]"); eauto; simplify_map_eq by simplify_pair_eq; eauto.
     { by rewrite !dom_insert; set_solver+. }
     { eapply mem_neq_implies_allow_load_map with (a := a) (pc_a := pc_a); eauto.
-      by simplify_map_eq. }
+      by simplify_map_eq by simplify_pair_eq. }
     iNext. iIntros (regs' retv) "(#Hspec & Hmem & Hmap)".
     iDestruct "Hspec" as %Hspec.
 
     destruct Hspec as [ | * Hfail ].
      { (* Success *)
        iApply "Hφ".
-       destruct H4 as [Hrr2 _]. simplify_map_eq.
+       destruct H4 as [Hrr2 _]. simplify_map_eq by simplify_pair_eq.
        iDestruct (memMap_resource_2ne with "Hmem") as "[Hpc_a Ha]";auto.
        incrementPC_inv.
-       simplify_map_eq.
+       simplify_map_eq by simplify_pair_eq.
        rewrite insert_insert insert_insert.
        iDestruct (regs_of_map_2 with "[$Hmap]") as "[HPC Hr2]"; eauto. iFrame. }
      { (* Failure (contradiction) *)
-       destruct Hfail; try incrementPC_inv; simplify_map_eq; eauto.
+       destruct Hfail; try incrementPC_inv; simplify_map_eq by simplify_pair_eq; eauto.
        destruct o. all: congruence. }
   Qed.
 
@@ -662,42 +668,44 @@ Section cap_lang_rules.
     - by iDestruct "HH" as "[HH _]".
   Qed.
 
-  Lemma wp_load_success_fromPC E r1 pc_p pc_b pc_e pc_a pc_a' w w'' dq :
+  Lemma wp_load_success_fromPC E i r1 pc_p pc_b pc_e pc_a pc_a' w w'' dq :
     decodeInstrW w = Load r1 PC →
     isCorrectPC (WCap pc_p pc_b pc_e pc_a) →
     (pc_a + 1)%a = Some pc_a' →
 
-    {{{ ▷ PC ↦ᵣ WCap pc_p pc_b pc_e pc_a
+    {{{ ▷ (i, PC) ↦ᵣ WCap pc_p pc_b pc_e pc_a
           ∗ ▷ pc_a ↦ₐ{dq} w
-          ∗ ▷ r1 ↦ᵣ w'' }}}
-      Instr Executable @ E
-      {{{ RET NextIV;
-          PC ↦ᵣ WCap pc_p pc_b pc_e pc_a'
+          ∗ ▷ (i, r1) ↦ᵣ w'' }}}
+      (i, Instr Executable) @ E
+      {{{ RET (i, NextIV);
+          (i, PC) ↦ᵣ WCap pc_p pc_b pc_e pc_a'
              ∗ pc_a ↦ₐ{dq} w
-             ∗ r1 ↦ᵣ w }}}.
+             ∗ (i, r1) ↦ᵣ w }}}.
   Proof.
     iIntros (Hinstr Hvpc Hpca' φ)
             "(>HPC & >Hi & >Hr1) Hφ".
     iDestruct (map_of_regs_2 with "HPC Hr1") as "[Hmap %]".
     rewrite memMap_resource_1_dq.
-    iApply (wp_load with "[$Hmap $Hi]"); eauto; simplify_map_eq; eauto.
+    iApply (wp_load with "[$Hmap $Hi]"); eauto; simplify_map_eq by simplify_pair_eq; eauto.
     { by rewrite !dom_insert; set_solver+. }
     { eapply mem_eq_implies_allow_load_map with (a := pc_a); eauto.
-      by simplify_map_eq. }
+      by simplify_map_eq by simplify_pair_eq. }
     iNext. iIntros (regs' retv) "(#Hspec & Hmem & Hmap)".
     iDestruct "Hspec" as %Hspec.
 
     destruct Hspec as [ | * Hfail ].
      { (* Success *)
        iApply "Hφ".
-       destruct H3 as [Hrr2 _]. simplify_map_eq.
+       destruct H3 as [Hrr2 _]. simplify_map_eq by simplify_pair_eq.
        rewrite -memMap_resource_1_dq.
        incrementPC_inv.
-       simplify_map_eq.
-       rewrite insert_commute //= insert_insert insert_commute //= insert_insert.
+       simplify_map_eq by simplify_pair_eq.
+       rewrite (insert_commute _ (i, PC) (i, r1)) ; simplify_pair_eq.
+       rewrite insert_insert (insert_commute _ (i, r1) (i, PC)) ; simplify_pair_eq.
+       rewrite insert_insert ; simplify_pair_eq.
        iDestruct (regs_of_map_2 with "[$Hmap]") as "[HPC Hr1]"; eauto. iFrame. }
      { (* Failure (contradiction) *)
-       destruct Hfail; try incrementPC_inv; simplify_map_eq; eauto.
+       destruct Hfail; try incrementPC_inv; simplify_map_eq by simplify_pair_eq; eauto.
        apply isCorrectPC_ra_wb in Hvpc. apply andb_prop_elim in Hvpc as [Hra Hwb].
        destruct o; apply Is_true_false in H3. all: try congruence. done.
      }
