theories/rules/rules_Store.v
@@ -14,63 +14,64 @@ Section cap_lang_rules.
   Implicit Types r : RegName.
   Implicit Types v : cap_lang.val. 
   Implicit Types w : Word.
-  Implicit Types reg : gmap RegName Word.
+  Implicit Types reg : gmap (CoreN * RegName) Word.
   Implicit Types ms : gmap Addr Word.
 
-  Definition reg_allows_store (regs : Reg) (r : RegName) p b e a :=
-    regs !! r = Some (WCap p b e a) ∧
+  Definition reg_allows_store (i: CoreN) (regs : Reg) (r : RegName) p b e a :=
+    regs !! (i, r) = Some (WCap p b e a) ∧
     writeAllowed p = true ∧ withinBounds b e a = true.
 
-  Inductive Store_failure_store (regs: Reg) (r1 : RegName)(r2 : Z + RegName) (mem : gmap Addr Word):=
+  Inductive Store_failure_store (i: CoreN) (regs: Reg) (r1 : RegName)(r2 : Z + RegName) (mem : gmap Addr Word):=
   | Store_fail_const z:
-      regs !! r1 = Some(WInt z) ->
-      Store_failure_store regs r1 r2 mem
+      regs !! (i, r1) = Some(WInt z) ->
+      Store_failure_store i regs r1 r2 mem
   | Store_fail_bounds p b e a:
-      regs !! r1 = Some(WCap p b e a) ->
+      regs !! (i, r1) = Some(WCap p b e a) ->
       (writeAllowed p = false ∨ withinBounds b e a = false) →
-      Store_failure_store regs r1 r2 mem
+      Store_failure_store i regs r1 r2 mem
   | Store_fail_invalid_PC:
-      incrementPC (regs) = None ->
-      Store_failure_store regs r1 r2 mem
+      incrementPC (regs) i = None ->
+      Store_failure_store i regs r1 r2 mem
   .
 
   Inductive Store_failure_incr (regs: Reg) (r1 : RegName)(r2 : Z + RegName) (mem : gmap Addr Word):=
   .
 
   Inductive Store_spec
+    (i : CoreN)
     (regs: Reg) (r1 : RegName) (r2 : Z + RegName)
     (regs': Reg) (mem mem' : gmap Addr Word) : cap_lang.val → Prop
   :=
   | Store_spec_success p b e a storev oldv :
-      word_of_argument regs r2 = Some storev ->
-      reg_allows_store regs r1 p b e a  →
+      word_of_argument regs i r2 = Some storev ->
+      reg_allows_store i regs r1 p b e a  →
       mem !! a = Some oldv →
       mem' = (<[a := storev]> mem) →
-      incrementPC(regs) = Some regs' ->
-      Store_spec regs r1 r2 regs' mem mem' NextIV
+      incrementPC(regs) i = Some regs' ->
+      Store_spec i regs r1 r2 regs' mem mem' (i, NextIV)
   | Store_spec_failure_store :
       mem' = mem →
-      Store_failure_store regs r1 r2 mem ->
-      Store_spec regs r1 r2 regs' mem mem' FailedV.
+      Store_failure_store i regs r1 r2 mem ->
+      Store_spec i regs r1 r2 regs' mem mem' (i, FailedV).
 
-  Definition allow_store_map_or_true (r1 : RegName) (regs : Reg) (mem : gmap Addr Word):=
+  Definition allow_store_map_or_true (i: CoreN) (r1 : RegName) (regs : Reg) (mem : gmap Addr Word):=
     ∃ p b e a,
-      read_reg_inr regs r1 p b e a ∧ 
-      if decide (reg_allows_store regs r1 p b e a) then
+      read_reg_inr regs i r1 p b e a ∧
+      if decide (reg_allows_store i regs r1 p b e a) then
         ∃ w, mem !! a = Some w
       else True.
 
   Lemma allow_store_implies_storev:
-    ∀ (r1 : RegName)(r2 : Z + RegName) (mem0 : gmap Addr Word) (r : Reg) (p : Perm) (b e a : Addr) storev,
-      allow_store_map_or_true r1 r mem0
-      → r !! r1 = Some (WCap p b e a)
-      → word_of_argument r r2 = Some storev
+    ∀ (i: CoreN) (r1 : RegName)(r2 : Z + RegName) (mem0 : gmap Addr Word) (r : Reg) (p : Perm) (b e a : Addr) storev,
+      allow_store_map_or_true i r1 r mem0
+      → r !! (i, r1) = Some (WCap p b e a)
+      → word_of_argument r i r2 = Some storev
       → writeAllowed p = true
       → withinBounds b e a = true
       → ∃ (storev : Word),
           mem0 !! a = Some storev.
   Proof.
-    intros r1 r2 mem0 r p b e a storev HaStore Hr2v Hwoa Hwa Hwb.
+    intros i r1 r2 mem0 r p b e a storev HaStore Hr2v Hwoa Hwa Hwb.
     unfold allow_store_map_or_true in HaStore.
     destruct HaStore as (?&?&?&?&[Hrr | Hrl]&Hwo).
     - assert (Hrr' := Hrr).
@@ -83,12 +84,12 @@ Section cap_lang_rules.
   Qed.
 
   Lemma mem_eq_implies_allow_store_map:
-    ∀ (regs : Reg)(mem : gmap Addr Word)(r1 : RegName)(w : Word) p b e a,
+    ∀ (i: CoreN)(regs : Reg)(mem : gmap Addr Word)(r1 : RegName)(w : Word) p b e a,
       mem = <[a:=w]> ∅
-      → regs !! r1 = Some (WCap p b e a)
-      → allow_store_map_or_true r1 regs mem.
+      → regs !! (i, r1) = Some (WCap p b e a)
+      → allow_store_map_or_true i r1 regs mem.
   Proof.
-    intros regs mem r1 w p b e a Hmem Hrr2.
+    intros i regs mem r1 w p b e a Hmem Hrr2.
     exists p,b,e,a; split.
     - left. by simplify_map_eq.
     - case_decide; last done.
@@ -96,14 +97,14 @@ Section cap_lang_rules.
   Qed.
 
   Lemma mem_neq_implies_allow_store_map:
-    ∀ (regs : Reg)(mem : gmap Addr Word)(r1 : RegName)(pc_a : Addr)
+    ∀ (i: CoreN)(regs : Reg)(mem : gmap Addr Word)(r1 : RegName)(pc_a : Addr)
       (w w' : Word) p b e a,
       a ≠ pc_a
       → mem = <[pc_a:=w]> (<[a:=w']> ∅)
-      → regs !! r1 = Some (WCap p b e a)
-      → allow_store_map_or_true r1 regs mem.
+      → regs !! (i, r1) = Some (WCap p b e a)
+      → allow_store_map_or_true i r1 regs mem.
   Proof.
-    intros regs mem r1 pc_a w w' p b e a H4 Hrr2.
+    intros i regs mem r1 pc_a w w' p b e a H4 Hrr2.
     exists p,b,e,a; split.
     - left. by simplify_map_eq.
     - case_decide; last done.
@@ -111,35 +112,35 @@ Section cap_lang_rules.
   Qed.
 
   Lemma mem_implies_allow_store_map:
-    ∀ (regs : Reg)(mem : gmap Addr Word)(r1 : RegName)(pc_a : Addr)
+    ∀ (i: CoreN)(regs : Reg)(mem : gmap Addr Word)(r1 : RegName)(pc_a : Addr)
       (w w' : Word) p b e a,
       (if (a =? pc_a)%a
        then mem = <[pc_a:=w]> ∅
        else mem = <[pc_a:=w]> (<[a:=w']> ∅))
-      → regs !! r1 = Some (WCap p b e a)
-      → allow_store_map_or_true r1 regs mem.
+      → regs !! (i, r1) = Some (WCap p b e a)
+      → allow_store_map_or_true i r1 regs mem.
   Proof.
-    intros regs mem r1 pc_a w w' p b e a H4 Hrr2.
+    intros i regs mem r1 pc_a w w' p b e a H4 Hrr2.
     destruct (a =? pc_a)%a eqn:Heq.
       + apply Z.eqb_eq, finz_to_z_eq in Heq. subst a. eapply mem_eq_implies_allow_store_map; eauto.
       + apply Z.eqb_neq in Heq.  eapply mem_neq_implies_allow_store_map; eauto. congruence.
   Qed.
 
-   Lemma wp_store Ep
+   Lemma wp_store Ep i
      pc_p pc_b pc_e pc_a
      r1 (r2 : Z + RegName) w mem regs :
    decodeInstrW w = Store r1 r2 →
    isCorrectPC (WCap pc_p pc_b pc_e pc_a) →
-   regs !! PC = Some (WCap pc_p pc_b pc_e pc_a) →
-   regs_of (Store r1 r2) ⊆ dom _ regs →
+   regs !! (i, PC) = Some (WCap pc_p pc_b pc_e pc_a) →
+   regs_of_core (Store r1 r2) i ⊆ dom _ regs →
    mem !! pc_a = Some w →
-   allow_store_map_or_true r1 regs mem →
+   allow_store_map_or_true i r1 regs mem →
 
    {{{ (▷ [∗ map] a↦w ∈ mem, a ↦ₐ w) ∗
        ▷ [∗ map] k↦y ∈ regs, k ↦ᵣ y }}}
-     Instr Executable @ Ep
+     (i, Instr Executable) @ Ep
    {{{ regs' mem' retv, RET retv;
-       ⌜ Store_spec regs r1 r2 regs' mem mem' retv⌝ ∗
+       ⌜ Store_spec i regs r1 r2 regs' mem mem' retv⌝ ∗
          ([∗ map] a↦w ∈ mem', a ↦ₐ w) ∗
          [∗ map] k↦y ∈ regs', k ↦ᵣ y }}}.
    Proof.
@@ -151,25 +152,25 @@ Section cap_lang_rules.
      (* Derive necessary register values in r *)
      pose proof (lookup_weaken _ _ _ _ HPC Hregs).
      specialize (indom_regs_incl _ _ _ Dregs Hregs) as Hri. unfold regs_of in Hri.
-     feed destruct (Hri r1) as [r1v [Hr'1 Hr1]]. by set_solver+.
+     feed destruct (Hri i r1) as [r1v [Hr'1 Hr1]]. by set_solver+.
      iDestruct (gen_mem_valid_inSepM mem m with "Hm Hmem") as %Hma; eauto.
 
      iModIntro.
      iSplitR. by iPureIntro; apply normal_always_head_reducible.
      iNext. iIntros (e2 σ2 efs Hpstep).
      apply prim_step_exec_inv in Hpstep as (-> & -> & (c & -> & Hstep)).
-     iSplitR; auto. eapply step_exec_inv in Hstep; eauto.
+     iSplitR; auto. eapply core_step_exec_inv in Hstep; eauto.
 
      unfold exec in Hstep. simpl in Hstep.
      rewrite Hr1 in Hstep.
 
      (* Now we start splitting on the different cases in the Store spec, and prove them one at a time *)
 
-     destruct (word_of_argument regs r2) as [ storev | ] eqn:HSV.
+     destruct (word_of_argument regs i r2) as [ storev | ] eqn:HSV.
      2: {
        destruct r2 as [z | r2].
        - cbn in HSV; inversion HSV.
-       - destruct (Hri r2) as [r0v [Hr0 _] ]. by set_solver+.
+       - destruct (Hri i r2) as [r0v [Hr0 _] ]. rewrite /regs_of_core; by set_solver+.
          cbn in HSV. rewrite Hr0 in HSV. inversion HSV.
      }
      apply (word_of_arg_mono _ r) in HSV as HSV'; auto. rewrite HSV' in Hstep. cbn in Hstep.
@@ -190,14 +191,14 @@ Section cap_lang_rules.
      apply andb_true_iff in HWA; destruct HWA as (Hwa & Hwb).
 
      (* Prove that a is in the memory map now, otherwise we cannot continue *)
-     pose proof (allow_store_implies_storev r1 r2 mem regs p b e a storev) as (oldv & Hmema); auto.
+     pose proof (allow_store_implies_storev i r1 r2 mem regs p b e a storev) as (oldv & Hmema); auto.
 
      (* Given this, prove that a is also present in the memory itself *)
      iDestruct (gen_mem_valid_inSepM mem m a oldv with "Hm Hmem" ) as %Hma' ; auto.
 
-      destruct (incrementPC regs ) as [ regs' |] eqn:Hregs'.
+      destruct (incrementPC regs i) as [ regs' |] eqn:Hregs'.
       2: { (* Failure: the PC could not be incremented correctly *)
-        assert (incrementPC r = None).
+        assert (incrementPC r i = None).
         { eapply incrementPC_overflow_mono; first eapply Hregs'; eauto. }
         rewrite incrementPC_fail_updatePC /= in Hstep; auto.
         inversion Hstep.
@@ -205,35 +206,38 @@ Section cap_lang_rules.
         iPureIntro. eapply Store_spec_failure_store;eauto. by constructor.
       }
 
-      iMod ((gen_mem_update_inSepM _ _ a) with "Hm Hmem") as "[Hm Hmem]"; eauto.
+      iMod ((gen_mem_update_inSepM _ _ a) with "Hm Hmem") as "[Hm Hmem]" ; eauto.
 
      (* Success *)
       rewrite /update_mem /= in Hstep.
-      eapply (incrementPC_success_updatePC _ (<[a:=storev]> m)) in Hregs'
+      Unshelve.
+      eapply (incrementPC_success_updatePC _ i (<[a:=storev]> m) ) in Hregs'
         as (p1 & g1 & b1 & e1 & a1 & a_pc1 & HPC'' & HuPC & ->).
-      eapply (updatePC_success_incl _ (<[a:=storev]> m)) in HuPC. 2: by eauto.
+      eapply (updatePC_success_incl i _ (<[a:=storev]> m)) in HuPC. 2: by eauto.
+
       rewrite HuPC in Hstep; clear HuPC; inversion Hstep; clear Hstep; subst c σ2. cbn.
 
       iFrame.
-      iMod ((gen_heap_update_inSepM _ _ PC) with "Hr Hmap") as "[Hr Hmap]"; eauto.
+      iMod ((gen_heap_update_inSepM _ _ (i, PC)) with "Hr Hmap") as "[Hr Hmap]"; eauto.
       iFrame. iModIntro. iApply "Hφ". iFrame.
       iPureIntro. eapply Store_spec_success; eauto.
         * split; auto. exact Hr'1. all: auto.
-        * unfold incrementPC. rewrite a_pc1 HPC''. 
+        * unfold incrementPC. rewrite a_pc1 HPC''.
       Unshelve. all: auto.
    Qed.
 
-  Lemma wp_store_success_z_PC E pc_p pc_b pc_e pc_a pc_a' w z :
+  Lemma wp_store_success_z_PC E i pc_p pc_b pc_e pc_a pc_a' w z :
      decodeInstrW w = Store PC (inl z) →
      isCorrectPC (WCap pc_p pc_b pc_e pc_a) →
      (pc_a + 1)%a = Some pc_a' →
      writeAllowed pc_p = true →
 
-     {{{ ▷ PC ↦ᵣ WCap pc_p pc_b pc_e pc_a
+     {{{ ▷ (i, PC) ↦ᵣ WCap pc_p pc_b pc_e pc_a
            ∗ ▷ pc_a ↦ₐ w }}}
-       Instr Executable @ E
-       {{{ RET NextIV;
-           PC ↦ᵣ WCap pc_p pc_b pc_e pc_a'
+       (i, Instr Executable) @ E
+
+       {{{ RET (i, NextIV);
+           (i, PC) ↦ᵣ WCap pc_p pc_b pc_e pc_a'
               ∗ pc_a ↦ₐ (WInt z) }}}.
   Proof.
     iIntros (Hinstr Hvpc Hpca' Hwa φ)
@@ -241,82 +245,86 @@ Section cap_lang_rules.
     iDestruct (map_of_regs_1 with "HPC") as "Hmap".
     iDestruct (memMap_resource_1 with "Hi") as "Hmem".
 
-    iApply (wp_store with "[$Hmap $Hmem]"); eauto; simplify_map_eq; eauto.
+    iApply (wp_store with "[$Hmap $Hmem]"); eauto; simplify_map_eq by simplify_pair_eq; eauto.
     { by rewrite !dom_insert; set_solver+. }
-    { eapply mem_eq_implies_allow_store_map; eauto. }
+    { eapply mem_eq_implies_allow_store_map; simplify_map_eq by simplify_pair_eq
+      ; eauto. }
     iNext. iIntros (regs' mem' retv) "(#Hspec & Hmem & Hmap)".
     iDestruct "Hspec" as %Hspec.
 
     destruct Hspec. 
      { (* Success *)
        iApply "Hφ".
-       destruct H3 as [Hrr2 _]. simplify_map_eq.
+       destruct H3 as [Hrr2 _]. simplify_map_eq by simplify_pair_eq.
        rewrite memMap_resource_1.
        incrementPC_inv.
-       simplify_map_eq.
+       simplify_map_eq by simplify_pair_eq.
        rewrite !insert_insert.
        iDestruct (regs_of_map_1 with "[$Hmap]") as "HPC"; eauto. iFrame. }
      { (* Failure (contradiction) *)
-       destruct H3; try incrementPC_inv; simplify_map_eq; eauto.
+       destruct H3; try incrementPC_inv; simplify_map_eq by simplify_pair_eq; eauto.
        apply isCorrectPC_ra_wb in Hvpc. apply andb_prop_elim in Hvpc as [_ Hwb].
        destruct o; last apply Is_true_false in H2. all:try congruence. done.
      }
    Qed.
 
-   Lemma wp_store_success_reg_PC E src wsrc pc_p pc_b pc_e pc_a pc_a' w :
+   Lemma wp_store_success_reg_PC E i src wsrc pc_p pc_b pc_e pc_a pc_a' w :
      decodeInstrW w = Store PC (inr src) →
      isCorrectPC (WCap pc_p pc_b pc_e pc_a) →
      (pc_a + 1)%a = Some pc_a' →
      writeAllowed pc_p = true →
 
-     {{{ ▷ PC ↦ᵣ WCap pc_p pc_b pc_e pc_a
+     {{{ ▷ (i, PC) ↦ᵣ WCap pc_p pc_b pc_e pc_a
            ∗ ▷ pc_a ↦ₐ w
-           ∗ ▷ src ↦ᵣ wsrc }}}
-       Instr Executable @ E
-       {{{ RET NextIV;
-           PC ↦ᵣ WCap pc_p pc_b pc_e pc_a'
+           ∗ ▷ (i, src) ↦ᵣ wsrc }}}
+       (i, Instr Executable) @ E
+
+       {{{ RET (i, NextIV);
+           (i, PC) ↦ᵣ WCap pc_p pc_b pc_e pc_a'
               ∗ pc_a ↦ₐ wsrc
-              ∗ src ↦ᵣ wsrc }}}.
+              ∗ (i, src) ↦ᵣ wsrc }}}.
    Proof.
      iIntros (Hinstr Hvpc Hpca' Hwa φ)
             "(>HPC & >Hi & >Hsrc) Hφ".
      iDestruct (map_of_regs_2 with "HPC Hsrc") as "[Hmap %]".
      iDestruct (memMap_resource_1 with "Hi") as "Hmem".
 
-    iApply (wp_store with "[$Hmap $Hmem]"); eauto; simplify_map_eq; eauto.
-    { by rewrite !dom_insert; set_solver+. }
+    iApply (wp_store with "[$Hmap $Hmem]"); eauto; simplify_map_eq by simplify_pair_eq; eauto.
+    { rewrite !dom_insert /regs_of_core /regs_of /regs_of_argument
+      ; set_solver+. }
     { eapply mem_eq_implies_allow_store_map; eauto.
-      all: by simplify_map_eq. }
+      all: by simplify_map_eq by simplify_pair_eq. }
     iNext. iIntros (regs' mem' retv) "(#Hspec & Hmem & Hmap)".
     iDestruct "Hspec" as %Hspec.
 
     destruct Hspec. 
      { (* Success *)
        iApply "Hφ".
-       destruct H4 as [Hrr2 _]. simplify_map_eq.
+       destruct H4 as [Hrr2 _]. simplify_map_eq by simplify_pair_eq.
        rewrite memMap_resource_1.
        incrementPC_inv.
-       simplify_map_eq.
+       simplify_map_eq by simplify_pair_eq.
        do 2 rewrite insert_insert.
        iDestruct (regs_of_map_2 with "[$Hmap]") as "[HPC Hsrc]"; eauto. iFrame. }
      { (* Failure (contradiction) *)
-       destruct H4; try incrementPC_inv; simplify_map_eq; eauto.
+       destruct H4; try incrementPC_inv; simplify_map_eq by simplify_pair_eq; eauto.
        apply isCorrectPC_ra_wb in Hvpc. apply andb_prop_elim in Hvpc as [_ Hwb].
        destruct o; last apply Is_true_false in H3. congruence. done. congruence.
      }
     Qed.
 
-   Lemma wp_store_success_reg_PC_same E pc_p pc_b pc_e pc_a pc_a' w w' :
+   Lemma wp_store_success_reg_PC_same E i pc_p pc_b pc_e pc_a pc_a' w w' :
      decodeInstrW w = Store PC (inr PC) →
      isCorrectPC (WCap pc_p pc_b pc_e pc_a) →
      (pc_a + 1)%a = Some pc_a' →
      writeAllowed pc_p = true →
 
-     {{{ ▷ PC ↦ᵣ WCap pc_p pc_b pc_e pc_a
+     {{{ ▷ (i, PC) ↦ᵣ WCap pc_p pc_b pc_e pc_a
            ∗ ▷ pc_a ↦ₐ w }}}
-       Instr Executable @ E
-       {{{ RET NextIV;
-           PC ↦ᵣ WCap pc_p pc_b pc_e pc_a'
+       (i, Instr Executable) @ E
+
+       {{{ RET (i, NextIV);
+           (i, PC) ↦ᵣ WCap pc_p pc_b pc_e pc_a'
               ∗ pc_a ↦ₐ WCap pc_p pc_b pc_e pc_a }}}.
    Proof.
      iIntros (Hinstr Hvpc Hpca' Hwa φ)
@@ -324,92 +332,96 @@ Section cap_lang_rules.
      iDestruct (map_of_regs_1 with "HPC") as "Hmap".
      iDestruct (memMap_resource_1 with "Hi") as "Hmem".
 
-    iApply (wp_store with "[$Hmap $Hmem]"); eauto; simplify_map_eq; eauto.
-    { by rewrite !dom_insert; set_solver+. }
+    iApply (wp_store with "[$Hmap $Hmem]"); eauto; simplify_map_eq by simplify_pair_eq; eauto.
+    { rewrite !dom_insert /regs_of_core /regs_of /regs_of_argument
+      ; set_solver+. }
     { eapply mem_eq_implies_allow_store_map; eauto.
-      all: by simplify_map_eq. }
+      all: by simplify_map_eq by simplify_pair_eq. }
     iNext. iIntros (regs' mem' retv) "(#Hspec & Hmem & Hmap)".
     iDestruct "Hspec" as %Hspec.
 
     destruct Hspec. 
      { (* Success *)
        iApply "Hφ".
-       destruct H3 as [Hrr2 _]. simplify_map_eq.
+       destruct H3 as [Hrr2 _]. simplify_map_eq by simplify_pair_eq.
        rewrite memMap_resource_1.
        incrementPC_inv.
-       simplify_map_eq.
+       simplify_map_eq by simplify_pair_eq.
        do 2 rewrite insert_insert.
        iDestruct (regs_of_map_1 with "[$Hmap]") as "HPC"; eauto. iFrame. }
       { (* Failure (contradiction) *)
-       destruct H3; try incrementPC_inv; simplify_map_eq; eauto.
+       destruct H3; try incrementPC_inv; simplify_map_eq by simplify_pair_eq; eauto.
        apply isCorrectPC_ra_wb in Hvpc. apply andb_prop_elim in Hvpc as [_ Hwb].
        destruct o; last apply Is_true_false in H2. congruence. done. congruence.
      }
     Qed.
 
-   Lemma wp_store_success_same E pc_p pc_b pc_e pc_a pc_a' w dst z w'
+   Lemma wp_store_success_same E i pc_p pc_b pc_e pc_a pc_a' w dst z w'
          p b e :
      decodeInstrW w = Store dst (inl z) →
      isCorrectPC (WCap pc_p pc_b pc_e pc_a) →
      (pc_a + 1)%a = Some pc_a' →
      writeAllowed p = true → withinBounds b e pc_a = true →
 
-     {{{ ▷ PC ↦ᵣ WCap pc_p pc_b pc_e pc_a
+     {{{ ▷ (i, PC) ↦ᵣ WCap pc_p pc_b pc_e pc_a
            ∗ ▷ pc_a ↦ₐ w
-           ∗ ▷ dst ↦ᵣ WCap p b e pc_a }}}
-       Instr Executable @ E
-       {{{ RET NextIV;
-           PC ↦ᵣ WCap pc_p pc_b pc_e pc_a'
+           ∗ ▷ (i, dst) ↦ᵣ WCap p b e pc_a }}}
+       (i, Instr Executable) @ E
+
+       {{{ RET (i, NextIV);
+           (i, PC) ↦ᵣ WCap pc_p pc_b pc_e pc_a'
               ∗ pc_a ↦ₐ (WInt z)
-              ∗ dst ↦ᵣ WCap p b e pc_a }}}.
+              ∗ (i, dst) ↦ᵣ WCap p b e pc_a }}}.
     Proof.
      iIntros (Hinstr Hvpc Hpca' Hwa Hwb φ)
             "(>HPC & >Hi & >Hdst) Hφ".
      iDestruct (map_of_regs_2 with "HPC Hdst") as "[Hmap %]".
      iDestruct (memMap_resource_1 with "Hi") as "Hmem".
 
-    iApply (wp_store _ pc_p with "[$Hmap $Hmem]"); eauto; simplify_map_eq; eauto.
-    { by rewrite !dom_insert; set_solver+. }
+    iApply (wp_store _ i pc_p with "[$Hmap $Hmem]"); eauto; simplify_map_eq by simplify_pair_eq; eauto.
+    { rewrite !dom_insert /regs_of_core /regs_of /regs_of_argument
+      ; set_solver+. }
     { eapply mem_eq_implies_allow_store_map; eauto.
-      all: by simplify_map_eq. }
+      all: by simplify_map_eq by simplify_pair_eq. }
     iNext. iIntros (regs' mem' retv) "(#Hspec & Hmem & Hmap)".
     iDestruct "Hspec" as %Hspec.
 
     destruct Hspec. 
      { (* Success *)
        iApply "Hφ".
-       destruct H4 as [Hrr2 _]. simplify_map_eq.
+       destruct H4 as [Hrr2 _]. simplify_map_eq by simplify_pair_eq.
        rewrite memMap_resource_1.
        incrementPC_inv.
-       simplify_map_eq.
+       simplify_map_eq by simplify_pair_eq.
        do 2 rewrite insert_insert.
        iDestruct (regs_of_map_2 with "[$Hmap]") as "[HPC Hsrc]"; eauto. iFrame. }
      { (* Failure (contradiction) *)
-       destruct H4; try incrementPC_inv; simplify_map_eq; eauto.
+       destruct H4; try incrementPC_inv; simplify_map_eq by simplify_pair_eq; eauto.
        destruct o. all: congruence.
      }
      Qed.
 
-   Lemma wp_store_success_reg' E pc_p pc_b pc_e pc_a pc_a' w dst w'
+   Lemma wp_store_success_reg' E i pc_p pc_b pc_e pc_a pc_a' w dst w'
          p b e a :
       decodeInstrW w = Store dst (inr PC) →
      isCorrectPC (WCap pc_p pc_b pc_e pc_a) →
      (pc_a + 1)%a = Some pc_a' →
      writeAllowed p = true → withinBounds b e a = true →
 
-     {{{ ▷ PC ↦ᵣ WCap pc_p pc_b pc_e pc_a
+     {{{ ▷ (i, PC) ↦ᵣ WCap pc_p pc_b pc_e pc_a
            ∗ ▷ pc_a ↦ₐ w
-           ∗ ▷ dst ↦ᵣ WCap p b e a
+           ∗ ▷ (i, dst) ↦ᵣ WCap p b e a
            ∗ if (a =? pc_a)%a
              then emp
              else ▷ a ↦ₐ w' }}}
-       Instr Executable @ E
-       {{{ RET NextIV;
-           PC ↦ᵣ WCap pc_p pc_b pc_e pc_a'
+       (i, Instr Executable) @ E
+
+       {{{ RET (i, NextIV);
+           (i, PC) ↦ᵣ WCap pc_p pc_b pc_e pc_a'
               ∗ pc_a ↦ₐ (if (a =? pc_a)%a
                          then (WCap pc_p pc_b pc_e pc_a)
                          else w)
-              ∗ dst ↦ᵣ WCap p b e a
+              ∗ (i, dst) ↦ᵣ WCap p b e a
               ∗ if (a =? pc_a)%a
                 then emp
                 else a ↦ₐ (WCap pc_p pc_b pc_e pc_a) }}}.
@@ -419,10 +431,11 @@ Section cap_lang_rules.
      iDestruct (map_of_regs_2 with "HPC Hdst") as "[Hmap %]".
      iDestruct (memMap_resource_2gen_clater _ _ _ _ (λ a w, a ↦ₐ w)%I  with "Hi Ha") as (mem) "[>Hmem %]".
 
-    iApply (wp_store with "[$Hmap $Hmem]"); eauto; simplify_map_eq; eauto.
-    { by rewrite !dom_insert; set_solver+. }
-    { destruct (a =? pc_a)%a; by simplify_map_eq. }
-    { eapply mem_implies_allow_store_map; eauto. all: by simplify_map_eq. }
+    iApply (wp_store with "[$Hmap $Hmem]"); eauto; simplify_map_eq by simplify_pair_eq; eauto.
+    { rewrite !dom_insert /regs_of_core /regs_of /regs_of_argument
+      ; set_solver+. }
+    { destruct (a =? pc_a)%a; by simplify_map_eq by simplify_pair_eq. }
+    { eapply mem_implies_allow_store_map; eauto. all: by simplify_map_eq by simplify_pair_eq. }
 
     iNext. iIntros (regs' mem' retv) "(#Hspec & Hmem & Hmap)".
     iDestruct "Hspec" as %Hspec.
@@ -430,29 +443,29 @@ Section cap_lang_rules.
     destruct Hspec. 
      { (* Success *)
        iApply "Hφ".
-       destruct H5 as [Hrr2 _]. simplify_map_eq.
+       destruct H5 as [Hrr2 _]. simplify_map_eq by simplify_pair_eq.
        destruct (a0 =? pc_a)%a eqn:Heq; subst mem.
        -  apply Z.eqb_eq, finz_to_z_eq in Heq. subst a0.
           rewrite insert_insert.
           rewrite memMap_resource_1.
           incrementPC_inv.
-          simplify_map_eq. rewrite insert_insert.
+          simplify_map_eq by simplify_pair_eq. rewrite insert_insert.
           iDestruct (regs_of_map_2 with "[$Hmap]") as "[HPC Hsrc]"; eauto. iFrame.
 
        - apply Z.eqb_neq in Heq.
          rewrite insert_commute; last congruence. rewrite insert_insert.
          iDestruct (memMap_resource_2ne with "Hmem") as "[Ha0 Hpc_a]"; first congruence.
          incrementPC_inv.
-         rewrite lookup_insert_ne in H6; last congruence. simplify_map_eq. rewrite insert_insert.
+         rewrite lookup_insert_ne in H6; last congruence. simplify_map_eq by simplify_pair_eq. rewrite insert_insert.
          iDestruct (regs_of_map_2 with "[$Hmap]") as "[HPC Hsrc]"; eauto. iFrame.
      }
      { (* Failure (contradiction) *)
-       destruct H5; try incrementPC_inv; simplify_map_eq; eauto.
+       destruct H5; try incrementPC_inv; simplify_map_eq by simplify_pair_eq; eauto.
        destruct o. all: try congruence.
      }
    Qed.
 
-   Lemma wp_store_success_reg_frominstr_same E pc_p pc_b pc_e pc_a pc_a' w dst w'
+   Lemma wp_store_success_reg_frominstr_same E i pc_p pc_b pc_e pc_a pc_a' w dst w'
          p b e :
       decodeInstrW w = Store dst (inr PC) →
      isCorrectPC (WCap pc_p pc_b pc_e pc_a) →
@@ -460,14 +473,15 @@ Section cap_lang_rules.
      writeAllowed p = true →
      withinBounds b e pc_a = true →
 
-     {{{ ▷ PC ↦ᵣ WCap pc_p pc_b pc_e pc_a
+     {{{ ▷ (i, PC) ↦ᵣ WCap pc_p pc_b pc_e pc_a
            ∗ ▷ pc_a ↦ₐ w
-           ∗ ▷ dst ↦ᵣ WCap p b e pc_a }}}
-       Instr Executable @ E
-       {{{ RET NextIV;
-           PC ↦ᵣ WCap pc_p pc_b pc_e pc_a'
+           ∗ ▷ (i, dst) ↦ᵣ WCap p b e pc_a }}}
+       (i, Instr Executable) @ E
+
+       {{{ RET (i, NextIV);
+           (i, PC) ↦ᵣ WCap pc_p pc_b pc_e pc_a'
               ∗ pc_a ↦ₐ WCap pc_p pc_b pc_e pc_a
-              ∗ dst ↦ᵣ WCap p b e pc_a }}}.
+              ∗ (i, dst) ↦ᵣ WCap p b e pc_a }}}.
    Proof.
      intros. iIntros "(HPC & Hpc_a & Hdst) Hφ".
      iApply (wp_store_success_reg' with "[$HPC $Hpc_a $Hdst]"); eauto.
@@ -476,7 +490,7 @@ Section cap_lang_rules.
      iApply "Hφ". iFrame. Unshelve. eauto.
    Qed.
 
-   Lemma wp_store_success_reg_frominstr E pc_p pc_b pc_e pc_a pc_a' w dst w'
+   Lemma wp_store_success_reg_frominstr E i pc_p pc_b pc_e pc_a pc_a' w dst w'
          p b e a :
       decodeInstrW w = Store dst (inr PC) →
      isCorrectPC (WCap pc_p pc_b pc_e pc_a) →
@@ -484,15 +498,16 @@ Section cap_lang_rules.
      writeAllowed p = true →
      withinBounds b e a = true →
 
-     {{{ ▷ PC ↦ᵣ WCap pc_p pc_b pc_e pc_a
+     {{{ ▷ (i, PC) ↦ᵣ WCap pc_p pc_b pc_e pc_a
            ∗ ▷ pc_a ↦ₐ w
-           ∗ ▷ dst ↦ᵣ WCap p b e a
+           ∗ ▷ (i, dst) ↦ᵣ WCap p b e a
            ∗ ▷ a ↦ₐ w' }}}
-       Instr Executable @ E
-       {{{ RET NextIV;
-           PC ↦ᵣ WCap pc_p pc_b pc_e pc_a'
+       (i, Instr Executable) @ E
+
+       {{{ RET (i, NextIV);
+           (i, PC) ↦ᵣ WCap pc_p pc_b pc_e pc_a'
               ∗ pc_a ↦ₐ w
-              ∗ dst ↦ᵣ WCap p b e a
+              ∗ (i, dst) ↦ᵣ WCap p b e a
               ∗ a ↦ₐ WCap pc_p pc_b pc_e pc_a }}}.
    Proof.
      intros. iIntros "(>HPC & >Hpc_a & >Hdst & >Ha) Hφ".
@@ -505,112 +520,117 @@ Section cap_lang_rules.
      iApply "Hφ". iFrame.
   Qed.
 
-   Lemma wp_store_success_reg_same' E pc_p pc_b pc_e pc_a pc_a' w dst
+   Lemma wp_store_success_reg_same' E i pc_p pc_b pc_e pc_a pc_a' w dst
          p b e :
      decodeInstrW w = Store dst (inr dst) →
      isCorrectPC (WCap pc_p pc_b pc_e pc_a) →
      (pc_a + 1)%a = Some pc_a' →
      writeAllowed p = true → withinBounds b e pc_a = true →
 
-     {{{ ▷ PC ↦ᵣ WCap pc_p pc_b pc_e pc_a
+     {{{ ▷ (i, PC) ↦ᵣ WCap pc_p pc_b pc_e pc_a
            ∗ ▷ pc_a ↦ₐ w
-           ∗ ▷ dst ↦ᵣ WCap p b e pc_a }}}
-       Instr Executable @ E
-       {{{ RET NextIV;
-           PC ↦ᵣ WCap pc_p pc_b pc_e pc_a'
+           ∗ ▷ (i, dst) ↦ᵣ WCap p b e pc_a }}}
+       (i, Instr Executable) @ E
+
+       {{{ RET (i, NextIV);
+           (i, PC) ↦ᵣ WCap pc_p pc_b pc_e pc_a'
               ∗ pc_a ↦ₐ WCap p b e pc_a
-              ∗ dst ↦ᵣ WCap p b e pc_a }}}.
+              ∗ (i, dst) ↦ᵣ WCap p b e pc_a }}}.
    Proof.
      iIntros (Hinstr Hvpc Hpca' Hwa Hwb φ)
             "(>HPC & >Hi & >Hdst) Hφ".
      iDestruct (map_of_regs_2 with "HPC Hdst") as "[Hmap %]".
      iDestruct (memMap_resource_1 with "Hi") as "Hmem".
 
-    iApply (wp_store _ pc_p with "[$Hmap $Hmem]"); eauto; simplify_map_eq; eauto.
-    { by rewrite !dom_insert; set_solver+. }
+    iApply (wp_store _ i pc_p with "[$Hmap $Hmem]"); eauto; simplify_map_eq by simplify_pair_eq; eauto.
+    { rewrite /regs_of_core /regs_of /regs_of_argument
+      ; set_solver+. }
     { eapply mem_eq_implies_allow_store_map; eauto.
-      all: by simplify_map_eq. }
+      all: by simplify_map_eq by simplify_pair_eq. }
     iNext. iIntros (regs' mem' retv) "(#Hspec & Hmem & Hmap)".
     iDestruct "Hspec" as %Hspec.
 
     destruct Hspec. 
      { (* Success *)
        iApply "Hφ".
-       destruct H4 as [Hrr2 _]. simplify_map_eq.
+       destruct H4 as [Hrr2 _]. simplify_map_eq by simplify_pair_eq.
        rewrite memMap_resource_1.
        incrementPC_inv.
-       simplify_map_eq.
+       simplify_map_eq by simplify_pair_eq.
        do 2 rewrite insert_insert.
        iDestruct (regs_of_map_2 with "[$Hmap]") as "[HPC Hsrc]"; eauto. iFrame. }
      { (* Failure (contradiction) *)
-       destruct H4; try incrementPC_inv; simplify_map_eq; eauto.
+       destruct H4; try incrementPC_inv; simplify_map_eq by simplify_pair_eq; eauto.
        destruct o. all: try congruence.
      }
    Qed.
 
-   Lemma wp_store_success_reg_same_a E pc_p pc_b pc_e pc_a pc_a' w dst src
+   Lemma wp_store_success_reg_same_a E i pc_p pc_b pc_e pc_a pc_a' w dst src
          p b e w'' :
       decodeInstrW w = Store dst (inr src) →
      isCorrectPC (WCap pc_p pc_b pc_e pc_a) →
      (pc_a + 1)%a = Some pc_a' →
      writeAllowed p = true → withinBounds b e pc_a = true →
 
-     {{{ ▷ PC ↦ᵣ WCap pc_p pc_b pc_e pc_a
+     {{{ ▷ (i, PC) ↦ᵣ WCap pc_p pc_b pc_e pc_a
            ∗ ▷ pc_a ↦ₐ w
-           ∗ ▷ src ↦ᵣ w''
-           ∗ ▷ dst ↦ᵣ WCap p b e pc_a }}}
-       Instr Executable @ E
-       {{{ RET NextIV;
-           PC ↦ᵣ WCap pc_p pc_b pc_e pc_a'
+           ∗ ▷ (i, src) ↦ᵣ w''
+           ∗ ▷ (i, dst) ↦ᵣ WCap p b e pc_a }}}
+       (i, Instr Executable) @ E
+
+       {{{ RET (i, NextIV);
+           (i, PC) ↦ᵣ WCap pc_p pc_b pc_e pc_a'
               ∗ pc_a ↦ₐ w''
-              ∗ src ↦ᵣ w''
-              ∗ dst ↦ᵣ WCap p b e pc_a}}}.
+              ∗ (i, src) ↦ᵣ w''
+              ∗ (i, dst) ↦ᵣ WCap p b e pc_a}}}.
    Proof.
      iIntros (Hinstr Hvpc Hpca' Hwa Hwb φ)
              "(>HPC & >Hi & >Hsrc & >Hdst) Hφ".
      iDestruct (map_of_regs_3 with "HPC Hsrc Hdst") as "[Hmap (%&%&%)]".
      iDestruct (memMap_resource_1 with "Hi") as "Hmem".
 
-    iApply (wp_store _ pc_p with "[$Hmap $Hmem]"); eauto; simplify_map_eq; eauto.
-    { by rewrite !dom_insert; set_solver+. }
+    iApply (wp_store _ i pc_p with "[$Hmap $Hmem]"); eauto; simplify_map_eq by simplify_pair_eq; eauto.
+    { rewrite !dom_insert /regs_of_core /regs_of /regs_of_argument
+      ; set_solver+. }
     { eapply mem_eq_implies_allow_store_map; eauto.
-      all: by simplify_map_eq. }
+      all: by simplify_map_eq by simplify_pair_eq. }
     iNext. iIntros (regs' mem' retv) "(#Hspec & Hmem & Hmap)".
     iDestruct "Hspec" as %Hspec.
 
     destruct Hspec. 
      { (* Success *)
        iApply "Hφ".
-       destruct H6 as [Hrr2 _]. simplify_map_eq.
+       destruct H6 as [Hrr2 _]. simplify_map_eq by simplify_pair_eq.
        rewrite memMap_resource_1.
        incrementPC_inv.
-       simplify_map_eq.
+       simplify_map_eq by simplify_pair_eq.
        do 2 rewrite insert_insert.
        iDestruct (regs_of_map_3 with "[$Hmap]") as "[HPC [Hsrc Hdst] ]"; eauto. iFrame. }
      { (* Failure (contradiction) *)
-       destruct H6; try incrementPC_inv; simplify_map_eq; eauto.
+       destruct H6; try incrementPC_inv; simplify_map_eq by simplify_pair_eq; eauto.
        destruct o. all: try congruence.
      }
    Qed.
 
-   Lemma wp_store_success_reg E pc_p pc_b pc_e pc_a pc_a' w dst src w'
+   Lemma wp_store_success_reg E i pc_p pc_b pc_e pc_a pc_a' w dst src w'
          p b e a w'' :
       decodeInstrW w = Store dst (inr src) →
      isCorrectPC (WCap pc_p pc_b pc_e pc_a) →
      (pc_a + 1)%a = Some pc_a' →
      writeAllowed p = true → withinBounds b e a = true →
 
-     {{{ ▷ PC ↦ᵣ WCap pc_p pc_b pc_e pc_a
+     {{{ ▷ (i, PC) ↦ᵣ WCap pc_p pc_b pc_e pc_a
            ∗ ▷ pc_a ↦ₐ w
-           ∗ ▷ src ↦ᵣ w''
-           ∗ ▷ dst ↦ᵣ WCap p b e a
+           ∗ ▷ (i, src) ↦ᵣ w''
+           ∗ ▷ (i, dst) ↦ᵣ WCap p b e a
            ∗ ▷ a ↦ₐ w' }}}
-       Instr Executable @ E
-       {{{ RET NextIV;
-           PC ↦ᵣ WCap pc_p pc_b pc_e pc_a'
+       (i, Instr Executable) @ E
+
+       {{{ RET (i, NextIV);
+           (i, PC) ↦ᵣ WCap pc_p pc_b pc_e pc_a'
               ∗ pc_a ↦ₐ w
-              ∗ src ↦ᵣ w''
-              ∗ dst ↦ᵣ WCap p b e a
+              ∗ (i, src) ↦ᵣ w''
+              ∗ (i, dst) ↦ᵣ WCap p b e a
               ∗ a ↦ₐ w'' }}}.
     Proof.
       iIntros (Hinstr Hvpc Hpca' Hwa Hwb φ)
@@ -618,45 +638,47 @@ Section cap_lang_rules.
     iDestruct (map_of_regs_3 with "HPC Hsrc Hdst") as "[Hmap (%&%&%)]".
     iDestruct (memMap_resource_2ne_apply with "Hi Hsrca") as "[Hmem %]"; auto.
 
-    iApply (wp_store _ pc_p with "[$Hmap $Hmem]"); eauto; simplify_map_eq; eauto.
-    { by rewrite !dom_insert; set_solver+. }
+    iApply (wp_store _ i pc_p with "[$Hmap $Hmem]"); eauto; simplify_map_eq by simplify_pair_eq; eauto.
+    { rewrite !dom_insert /regs_of_core /regs_of /regs_of_argument
+      ; set_solver+. }
     { eapply mem_neq_implies_allow_store_map with (a := a); eauto.
-      all: by simplify_map_eq. }
+      all: by simplify_map_eq by simplify_pair_eq. }
     iNext. iIntros (regs' mem' retv) "(#Hspec & Hmem & Hmap)".
     iDestruct "Hspec" as %Hspec.
 
     destruct Hspec. 
      { (* Success *)
        iApply "Hφ".
-       destruct H7 as [Hrr2 _]. simplify_map_eq.
+       destruct H7 as [Hrr2 _]. simplify_map_eq by simplify_pair_eq.
        rewrite insert_commute // insert_insert.
        iDestruct (memMap_resource_2ne with "Hmem") as "[Hpc_a Ha]";auto.
        incrementPC_inv.
-       simplify_map_eq.
+       simplify_map_eq by simplify_pair_eq.
        rewrite insert_insert.
        iDestruct (regs_of_map_3 with "[$Hmap]") as "[HPC [Hsrc Hdst] ]"; eauto. iFrame. }
      { (* Failure (contradiction) *)
-       destruct H7; try incrementPC_inv; simplify_map_eq; eauto.
+       destruct H7; try incrementPC_inv; simplify_map_eq by simplify_pair_eq; eauto.
        destruct o. all: try congruence.
      }
     Qed.
 
-   Lemma wp_store_success_reg_same E pc_p pc_b pc_e pc_a pc_a' w dst w'
+   Lemma wp_store_success_reg_same E i pc_p pc_b pc_e pc_a pc_a' w dst w'
          p b e a :
      decodeInstrW w = Store dst (inr dst) →
      isCorrectPC (WCap pc_p pc_b pc_e pc_a) →
      (pc_a + 1)%a = Some pc_a' →
      writeAllowed p = true → withinBounds b e a = true →
 
-     {{{ ▷ PC ↦ᵣ WCap pc_p pc_b pc_e pc_a
+     {{{ ▷ (i, PC) ↦ᵣ WCap pc_p pc_b pc_e pc_a
            ∗ ▷ pc_a ↦ₐ w
-           ∗ ▷ dst ↦ᵣ WCap p b e a
+           ∗ ▷ (i, dst) ↦ᵣ WCap p b e a
            ∗ ▷ a ↦ₐ w' }}}
-       Instr Executable @ E
-       {{{ RET NextIV;
-           PC ↦ᵣ WCap pc_p pc_b pc_e pc_a'
+       (i, Instr Executable) @ E
+
+       {{{ RET (i, NextIV);
+           (i, PC) ↦ᵣ WCap pc_p pc_b pc_e pc_a'
               ∗ pc_a ↦ₐ w
-              ∗ dst ↦ᵣ WCap p b e a
+              ∗ (i, dst) ↦ᵣ WCap p b e a
               ∗ a ↦ₐ WCap p b e a }}}.
    Proof.
     iIntros (Hinstr Hvpc Hpca' Hwa Hwb φ)
@@ -664,45 +686,47 @@ Section cap_lang_rules.
     iDestruct (map_of_regs_2 with "HPC Hdst") as "[Hmap %]".
     iDestruct (memMap_resource_2ne_apply with "Hi Hsrca") as "[Hmem %]"; auto.
 
-    iApply (wp_store _ pc_p with "[$Hmap $Hmem]"); eauto; simplify_map_eq; eauto.
-    { by rewrite !dom_insert; set_solver+. }
+    iApply (wp_store _ i pc_p with "[$Hmap $Hmem]"); eauto; simplify_map_eq by simplify_pair_eq; eauto.
+    { rewrite !dom_insert /regs_of_core /regs_of /regs_of_argument
+      ; set_solver+. }
     { eapply mem_neq_implies_allow_store_map with (a := a); eauto.
-      all: by simplify_map_eq. }
+      all: by simplify_map_eq by simplify_pair_eq. }
     iNext. iIntros (regs' mem' retv) "(#Hspec & Hmem & Hmap)".
     iDestruct "Hspec" as %Hspec.
 
     destruct Hspec. 
      { (* Success *)
        iApply "Hφ".
-       destruct H5 as [Hrr2 _]. simplify_map_eq.
+       destruct H5 as [Hrr2 _]. simplify_map_eq by simplify_pair_eq.
        rewrite insert_commute // insert_insert.
        iDestruct (memMap_resource_2ne with "Hmem") as "[Hpc_a Ha]";auto.
        incrementPC_inv.
-       simplify_map_eq.
+       simplify_map_eq by simplify_pair_eq.
        rewrite insert_insert.
        iDestruct (regs_of_map_2 with "[$Hmap]") as "[HPC Hdst]"; eauto. iFrame. }
      { (* Failure (contradiction) *)
-       destruct H5; try incrementPC_inv; simplify_map_eq; eauto.
+       destruct H5; try incrementPC_inv; simplify_map_eq by simplify_pair_eq; eauto.
        destruct o. all: try congruence.
      }
     Qed.
 
-   Lemma wp_store_success_z E pc_p pc_b pc_e pc_a pc_a' w dst z w'
+   Lemma wp_store_success_z E i pc_p pc_b pc_e pc_a pc_a' w dst z w'
          p b e a :
      decodeInstrW w = Store dst (inl z) →
      isCorrectPC (WCap pc_p pc_b pc_e pc_a) →
      (pc_a + 1)%a = Some pc_a' →
      writeAllowed p = true → withinBounds b e a = true →
 
-     {{{ ▷ PC ↦ᵣ WCap pc_p pc_b pc_e pc_a
+     {{{ ▷ (i, PC) ↦ᵣ WCap pc_p pc_b pc_e pc_a
            ∗ ▷ pc_a ↦ₐ w
-           ∗ ▷ dst ↦ᵣ WCap p b e a
+           ∗ ▷ (i, dst) ↦ᵣ WCap p b e a
            ∗ ▷ a ↦ₐ w' }}}
-       Instr Executable @ E
-       {{{ RET NextIV;
-           PC ↦ᵣ WCap pc_p pc_b pc_e pc_a'
+       (i, Instr Executable) @ E
+
+       {{{ RET (i, NextIV);
+           (i, PC) ↦ᵣ WCap pc_p pc_b pc_e pc_a'
               ∗ pc_a ↦ₐ w
-              ∗ dst ↦ᵣ WCap p b e a
+              ∗ (i, dst) ↦ᵣ WCap p b e a
               ∗ a ↦ₐ WInt z }}}.
    Proof.
      iIntros (Hinstr Hvpc Hpca' Hwa Hwb φ)
@@ -710,25 +734,25 @@ Section cap_lang_rules.
     iDestruct (map_of_regs_2 with "HPC Hdst") as "[Hmap %]".
     iDestruct (memMap_resource_2ne_apply with "Hi Hsrca") as "[Hmem %]"; auto.
 
-    iApply (wp_store _ pc_p with "[$Hmap $Hmem]"); eauto; simplify_map_eq; eauto.
+    iApply (wp_store _  i pc_p with "[$Hmap $Hmem]"); eauto; simplify_map_eq by simplify_pair_eq; eauto.
     { by rewrite !dom_insert; set_solver+. }
     { eapply mem_neq_implies_allow_store_map with (a := a); eauto.
-      all: by simplify_map_eq. }
+      all: by simplify_map_eq by simplify_pair_eq. }
     iNext. iIntros (regs' mem' retv) "(#Hspec & Hmem & Hmap)".
     iDestruct "Hspec" as %Hspec.
 
     destruct Hspec. 
      { (* Success *)
        iApply "Hφ".
-       destruct H5 as [Hrr2 _]. simplify_map_eq.
+       destruct H5 as [Hrr2 _]. simplify_map_eq by simplify_pair_eq.
        rewrite insert_commute // insert_insert.
        iDestruct (memMap_resource_2ne with "Hmem") as "[Hpc_a Ha]";auto.
        incrementPC_inv.
-       simplify_map_eq.
+       simplify_map_eq by simplify_pair_eq.
        rewrite insert_insert.
        iDestruct (regs_of_map_2 with "[$Hmap]") as "[HPC Hdst]"; eauto. iFrame. }
      { (* Failure (contradiction) *)
-       destruct H5; try incrementPC_inv; simplify_map_eq; eauto.
+       destruct H5; try incrementPC_inv; simplify_map_eq by simplify_pair_eq; eauto.
        destruct o. all: try congruence.
      }
     Qed.
